quotation/theories/ToTemplate/QuotationOf/Common/Kernames/Instances.v
@@ -1,0 +1,128 @@
+From MetaCoq.Quotation.ToTemplate Require Export Init.
+From MetaCoq.Common Require Import Kernames.
+From MetaCoq.Quotation.ToTemplate.QuotationOf.Coq.Structures Require Import Orders.Sig OrdersAlt.Sig OrdersFacts.Sig.
+From MetaCoq.Quotation.ToTemplate.QuotationOf.Coq.MSets Require Import MSetAVL.Sig MSetProperties.Sig.
+Import List.ListNotations.
+Local Open Scope list_scope.
+(*
+From Coq Require Import Lists.List.
+From MetaCoq.Common Require Import Kernames.
+From MetaCoq.Utils Require Import bytestring monad_utils.
+From MetaCoq.Utils Require Import utils MCList.
+From MetaCoq.Template Require Import Loader TemplateMonad.
+From MetaCoq.Template Require Import MonadBasicAst MonadAst TemplateMonad Ast Loader.
+Require Import Equations.Prop.Classes.
+Require Import Coq.Lists.List.
+Import ListNotations.
+
+Local Open Scope bs.
+Import MCMonadNotation.
+Import ListNotations.
+
+Local Set Primitive Projections.
+Local Unset Universe Minimization ToSet.
+Local Open Scope bs.
+Import MCMonadNotation.
+Set Printing Universes.
+MetaCoq Run (foo <- tmUnquote (tConst
+                                 (MPdot (MPdot (MPfile ["Kernames"; "Common"; "MetaCoq"]) "Kername") "OT",
+                                   "t") []);;
+             let '{| my_projT1 := ty ; my_projT2 := v |} := foo in
+             _ <- @tmDefinition "foo" _ (let x : ty := v in tt);;
+             _ <- @tmDefinition "bar" _ (let x : ty := v in tt);;
+             ret tt).
+Set Printing All.
+Print bar.
+Defined.
+  run_template_program (gr <- tmLocate1 "Kername.OT.t";;
+                        match gr with
+                        | ConstRef cr => v <- tmUnquote (tConst cr nil);;
+                                         ret (v, tConst cr nil)
+                        | _ => tmFail ""
+                        end) (fun v => pose v).
+
+MetaCoq Run (tmMakeQuotationOfModule everything None "KernameSetOrdProp.ME").
+ *)
+HERE
+Module qKername <: QuotationOfOrderedType Kername.
+  Module qOT <: QuotationOfOrderedTypeOrig Kername.OT.
+    MetaCoq Run (tmMakeQuotationOfModule everything None "Kername.OT").
+  End qOT.
+  MetaCoq Run (tmMakeQuotationOfModuleWorkAroundCoqBug17303 (all_submodules_except [["OT"]]%bs) (*None*) "Kername").
+End qKername.
+(*
+Module qKernameSet <: MSetAVL.QuotationOfMake Kername KernameSet.
+  Instance :debug_opt := true.
+  Set Printing Implicit. Set Printing Universes.
+  MetaCoq Run (tmMakeQuotationOfModule everything None "KernameSet").
+End qKernameSet.
+*)
+Module qKernameSetOrdProp <: QuotationOfOrdProperties KernameSet KernameSetOrdProp.
+  Module qME <: QuotationOfOrderedTypeFacts KernameSet.E KernameSetOrdProp.ME.
+    Set Printing Implicit. Set Printing Universes.
+    Instance: debug_opt := true.
+    MetaCoq Run (tmMakeQuotationOfModule everything None "KernameSetOrdProp.ME").
+  End qME.
+  Module qML. (* OrderedTypeLists(M.E). *)
+    MetaCoq Run (tmMakeQuotationOfModule everything None "KernameSetOrdProp.ML").
+  End qML.
+  Module qP <: QuotationOfWProperties KernameSet KernameSetOrdProp.P.
+    MetaCoq Run (tmMakeQuotationOfModule everything None "KernameSetOrdProp.ME").
+  End qP.
+  MetaCoq Run (tmMakeQuotationOfModule (all_submodules_except [["ME"]; ["ML"]; ["P"]]%bs) None "KernameSetOrdProp").
+
+
+  Module qME := Structures.QuotationOfOrderedTypeFacts KernameSet.E KernameSetOrdProp.ME qKername.
+  (*Module qML := QuotationOfOrderedTypeLists M.E F.ML.*)
+  Module qP <: MSets.QuotationOfWProperties KernameSet KernameSetOrdProp.P.
+    Module qDec <: MSets.QuotationOfWDecideOn Kername KernameSet KernameSetOrdProp.P.Dec.
+      Module qF <: MSets.QuotationOfWFactsOn Kername KernameSet KernameSetOrdProp.P.Dec.F.
+        Module F'. Include KernameSetOrdProp.P.Dec.F. End F'.
+        MetaCoq Run (Kernames_mp <- tmExtractBaseModPathFromMod "MetaCoq.Common.Kernames";; tmMakeQuotationOfModuleAndRebase false "F'" (MPdot (MPdot (MPdot (MPdot Kernames_mp "KernameSetOrdProp") "P") "Dec") "F")).
+      End qF.
+      Module qMSetDecideAuxiliary.
+        Module MSetDecideAuxiliary'. Include KernameSetOrdProp.P.Dec.MSetDecideAuxiliary. End MSetDecideAuxiliary'.
+        MetaCoq Run (Kernames_mp <- tmExtractBaseModPathFromMod "MetaCoq.Common.Kernames";; tmMakeQuotationOfModuleAndRebase false "MSetDecideAuxiliary'" (MPdot (MPdot (MPdot (MPdot Kernames_mp "KernameSetOrdProp") "P") "Dec") "MSetDecideAuxiliary")).
+      End qMSetDecideAuxiliary.
+    End qDec.
+    Module qFM <: MSets.QuotationOfWFactsOn Kername KernameSet KernameSetOrdProp.P.FM.
+      Module FM'. Include KernameSetOrdProp.P.FM. End FM'.
+      MetaCoq Run (Kernames_mp <- tmExtractBaseModPathFromMod "MetaCoq.Common.Kernames";; tmMakeQuotationOfModuleAndRebase false "FM'" (MPdot (MPdot (MPdot Kernames_mp "KernameSetOrdProp") "P") "FM")).
+    End qFM.
+    Module P'. Include KernameSetOrdProp.P. End P'.
+    MetaCoq Run (Kernames_mp <- tmExtractBaseModPathFromMod "MetaCoq.Common.Kernames";; tmMakeQuotationOfModuleAndRebase false "P'" (MPdot (MPdot Kernames_mp "KernameSetOrdProp") "P")).
+  End qP.
+  Module KernameSetOrdProp'. Include KernameSetOrdProp. End KernameSetOrdProp'.
+  MetaCoq Run (Kernames_mp <- tmExtractBaseModPathFromMod "MetaCoq.Common.Kernames";; tmMakeQuotationOfModuleAndRebase false "KernameSetOrdProp'" (MPdot Kernames_mp "KernameSetOrdProp")).
+End qKernameSetOrdProp.
+Module qKernameMap <: FMapAVL.QuotationOfMake Kername.OT KernameMap qKername.qOT.
+  Module qRaw.
+    Module qProofs.
+      Module qMX := Structures.QuotationOfOrderedTypeOrigFacts Kername.OT KernameMap.Raw.Proofs.MX qKername.qOT.
+      Module qPX := Structures.QuotationOfKeyOrderedTypeOrig Kername.OT KernameMap.Raw.Proofs.PX qKername.qOT.
+      Module qL <: FMapList.QuotationOfRaw Kername.OT KernameMap.Raw.Proofs.L qKername.qOT.
+        Module qMX := Structures.QuotationOfOrderedTypeOrigFacts Kername.OT KernameMap.Raw.Proofs.L.MX qKername.qOT.
+        Module qPX := Structures.QuotationOfKeyOrderedTypeOrig Kername.OT KernameMap.Raw.Proofs.L.PX qKername.qOT.
+        Module L'. Include KernameMap.Raw.Proofs.L. End L'.
+        MetaCoq Run (Kernames_mp <- tmExtractBaseModPathFromMod "MetaCoq.Common.Kernames";; tmMakeQuotationOfModuleAndRebase false "L'" (MPdot (MPdot (MPdot (MPdot Kernames_mp "KernameMap") "Raw") "Proofs") "L")).
+      End qL.
+      Module Proofs'. Include KernameMap.Raw.Proofs. End Proofs'.
+      MetaCoq Run (Kernames_mp <- tmExtractBaseModPathFromMod "MetaCoq.Common.Kernames";; tmMakeQuotationOfModuleAndRebase false "Proofs'" (MPdot (MPdot (MPdot Kernames_mp "KernameMap") "Raw") "Proofs")).
+    End qProofs.
+    Module Raw'. Include KernameMap.Raw. End Raw'.
+    MetaCoq Run (Kernames_mp <- tmExtractBaseModPathFromMod "MetaCoq.Common.Kernames";; tmMakeQuotationOfModuleAndRebase false "Raw'" (MPdot (MPdot Kernames_mp "KernameMap") "Raw")).
+  End qRaw.
+  Module KernameMap'. Include KernameMap. End KernameMap'.
+  MetaCoq Run (Kernames_mp <- tmExtractBaseModPathFromMod "MetaCoq.Common.Kernames";; tmMakeQuotationOfModuleAndRebase false "KernameMap'" (MPdot Kernames_mp "KernameMap")).
+End qKernameMap.
+Module qKernameMapFact.
+  Module qF <: QuotationOfWFacts_fun Kername.OT KernameMap KernameMapFact.F.
+    Module F'. Include KernameMapFact.F. End F'.
+    MetaCoq Run (Kernames_mp <- tmExtractBaseModPathFromMod "MetaCoq.Common.Kernames";; tmMakeQuotationOfModuleAndRebase false "F'" (MPdot (MPdot Kernames_mp "KernameMapFact") "F")).
+  End qF.
+End qKernameMapFact.
+
+Module QuoteKernameSet := MSets.QuoteMSetAVL Kername KernameSet KernameSetOrdProp qKername qKernameSet qKernameSetOrdProp.
+Export (hints) QuoteKernameSet.
+Module QuoteKernameMap := FSets.QuoteFMapAVL Kername.OT KernameMap KernameMapFact.F qKername.qOT qKernameMap qKernameMapFact.qF.
+Export (hints) QuoteKernameMap.
