quotation/theories/ToTemplate/QuotationOf/Coq/FSets/FMapFacts/Sig.v
@@ -1,0 +1,9 @@
+From Coq.FSets Require Import FMapFacts.
+From Coq.Structures Require Import Orders.
+From MetaCoq.Quotation.ToTemplate Require Export Init.
+
+Module Type WFacts_funSig (E : DecidableTypeOrig) (M : WSfun E) := Nop <+ WFacts_fun E M.
+
+Module Type QuotationOfWFacts_fun (E : DecidableTypeOrig) (M : WSfun E) (F : WFacts_funSig E M).
+  MetaCoq Run (tmDeclareQuotationOfModule everything (Some export) "F").
+End QuotationOfWFacts_fun.
